%!TEX program = xelatex
\documentclass[a4papers]{ctexart}
\usepackage{amsmath}
\usepackage{amssymb}
\usepackage{amsthm}
\usepackage{pgf}
\usepackage{tikz}
\usepackage{stmaryrd}
\usepackage{txfonts} 
\usepackage{ebproof}
\usetikzlibrary{arrows,automata}
% \usepackage[latin1]{inputenc} 
\usepackage{verbatim} 
\usepackage{geometry}
\geometry{left=2cm,right=2cm,top=1.8cm,bottom=1.5cm}

\newcommand{\btrue}{\ \boldsymbol{true}\ }
\newcommand{\bfalse}{\ \boldsymbol{false}\ }
\newcommand{\brem}{\ \boldsymbol{rem}\ }
\newcommand{\bif}{\ \boldsymbol{if}\ }
\newcommand{\belse}{\ \boldsymbol{else}\ }
\newcommand{\bthen}{\ \boldsymbol{then}\ }
\newcommand{\bwhile}{\ \boldsymbol{while}\ }
\newcommand{\bdo}{\ \boldsymbol{do}\ }
\newcommand{\bskip}{\ \boldsymbol{skip}\ }
\newcommand{\hello}{$HELLO$}
\newcommand{\hore}[3]{[#1]#2[#3]}
\newcommand{\horep}[3]{\{#1\}#2\{#3\}}
\newcommand{\tab}{\ \ \ \ }
\newcommand{\w}{\wedge }
\setlength{\parindent}{2em}

\setromanfont{Songti SC}
%\setromanfont{Heiti SC}

\title{FSPL -- Assignment 4}
\author{冯诗伟161220039}
\date{}
\begin{document}
\maketitle
\section*{3.1}
\begin{enumerate}
    \item $y=x^2$
    \item $y=z \wedge x=w $
    \item $a \le b \wedge y=ax$
    \item $\btrue$
    \item $\bfalse$
\end{enumerate}

\section*{3.2}
\noindent
The program $P$ is $c:=a\ ;d:=b;\bwhile(d>0) \bdo (r:=c \brem d;c:=d;d:=r)  $.\\
The loop invariant is $d\ge 0 \wedge gcd(c,d)=gcd(a,b) $.\\
Proof:
\begin{enumerate}
    \item $[a\ge0 \wedge b \ge 0 \wedge gcd(a,b)=gcd(a,b) ] \tab
            c:=a\tab [a\ge0 \wedge b \ge 0 \wedge gcd(c,b)=gcd(a,b) ]$ \hfill AS
    \item $[a\ge0 \wedge b \ge 0 \wedge gcd(c,b)=gcd(a,b) ] \tab
            d:=b\tab [d \ge 0 \wedge gcd(c,d)=gcd(a,b) ]$ \hfill AS
    \item $[a\ge0 \wedge b \ge 0 \wedge gcd(a,b)=gcd(a,b) ]
            c:=a;d:=b;[d \ge 0 \wedge gcd(c,d)=gcd(a,b) ]$ \hfill SC,1,2
    \item $[d\ge 0 \w gcd(c,d)=gcd(a,b) \w d>0 \w d=z ] r:=c \brem d 
            [d\ge 0 \w gcd(d,r)=gcd(a,b) \w d>0 \w d=z ]$               \hfill AS
    \item $[d\ge 0 \w gcd(d,r)=gcd(a,b) \w d>0 \w d=z ] \tab c:=d \tab 
            [d\ge 0 \w gcd(c,r)=gcd(a,b) \w d>0 \w d=z ]$               \hfill AS
    \item $[d\ge 0 \w gcd(c,r)=gcd(a,b) \w d>0 \w d=z ] \tab d:=r \tab
            [d\ge 0 \w gcd(c,d)=gcd(a,b) \w d>0 \w d<z ]$               \hfill AS
    \item $[d\ge 0 \w gcd(c,d)=gcd(a,b) \w d>0 \w d=z ]$\\
            $ r:=c \brem d ; c:=d $\\
            $[d\ge 0 \w gcd(c,r)=gcd(a,b) \w d>0 \w d=z ]$           \hfill SC,4,5
    \item $[d\ge 0 \w gcd(c,d)=gcd(a,b) \w d>0 \w d=z ]$\\
          $ r:=c \brem d ; c:=d ; d:=r$\\
          $ [d\ge 0 \w gcd(c,d)=gcd(a,b) \w d>0 \w d<z ] $          \hfill SC,7,6
    \item  $d\ge 0 \wedge gcd(c,d)=gcd(a,b) \w d > 0 \Rightarrow d\ge 0$
    \item  $[d\ge 0 \wedge gcd(c,d)=gcd(a,b)] $\\
             $\bwhile(d>0) \bdo (r:=c \brem d;c:=d;d:=r) $\\
            $[d\le 0 \w d \ge 0 \w gcd(c,d)=gcd(a,b)]$               \hfill WHT,8,9
    \item $[a\ge0 \wedge b \ge 0 \wedge gcd(a,b)=gcd(a,b) ]$\\
            $\tab c:=a;d:=b;\bwhile(d>0) \bdo (r:=c \brem d;c:=d;d:=r)$\\  
            $[d\le 0 \w d \ge 0 \w gcd(c,d)=gcd(a,b) ]$              \hfill SC 3,10
    \item  $[d\le 0 \w d \ge 0 \w gcd(c,d)=gcd(a,b) ]\Rightarrow [gcd(c,0)=gcd(a,b)]$
    \item $[a\ge0 \wedge b \ge 0 \wedge gcd(a,b)=gcd(a,b) ]$\\
           $c:=a;d:=b;\bwhile(d>0) \bdo (r:=c \brem d;c:=d;d:=r)$\\
            $[ gcd(c,0)=gcd(a,b) ]$                                 \hfill WC,11,12
    \item $gcd(c,0)=gcd(a,b) \Rightarrow c=gcd(a,b)$                  
    \item $[a\ge0 \wedge b \ge 0 \wedge gcd(a,b)=gcd(a,b) ]$\\
          $c:=a;d:=b;\bwhile(d>0) \bdo (r:=c \brem d;c:=d;d:=r)$\\ 
          $[c=gcd(a,b) ]$                                           \hfill WC,13,14
    \item $a\ge0 \wedge b \ge 0 \Rightarrow a\ge0 \wedge b \ge 0 \wedge gcd(a,b)=gcd(a,b)$
    \item $[a\ge0 \wedge b \ge 0  ]$\\
          $c:=a;d:=b;\bwhile(d>0) \bdo (r:=c \brem d;c:=d;d:=r)$\\ 
          $[c=gcd(a,b) ]$                                           \hfill SP,15,16
\end{enumerate}

\section*{3.4}
\noindent The loop invariant is $x \ge 0 \w y=y_0 + \frac{(x_0-x)(x_0+x-1)}{2}$.
\begin{enumerate}
    \item $[x\ge 0 \w y=y_0 + \frac{(x_0-x)(x_0+x-1)}{2} \w x\ne 0 \w x=z] x:=x-1
            [x\ge 0 \w y=y_0 + \frac{(x_0-x-1)(x_0+x)}{2}  \w x<z] $\hfill AS
    \item $[x\ge 0 \w y=y_0 + \frac{(x_0-x-1)(x_0+x)}{2}  \w x<z] \tab y:=y+x \tab 
            [x\ge 0 \w y=y_0 + \frac{(x_0+x-1)(x_0-x)}{2}  \w x<z]$\hfill AS
    \item $[x\ge 0 \w y=y_0 + \frac{(x_0-x)(x_0+x-1)}{2} \w x\ne 0 \w x=z]$\\
            $ x:=x-1;y:=y-x;$\\
            $ [x\ge 0 \w y=y_0 + \frac{(x_0-x)(x_0+x-1)}{2} \w x<z]$\hfill SC,1,2
    \item $x \ge 0 \w y=y_0 + \frac{(x_0-x)(x_0+x-1)}{2} \w x\ne 0 \Rightarrow x\ge 0$
    \item $[x \ge 0 \w y=y_0 + \frac{(x_0-x)(x_0+x-1)}{2}]$\\
           $\bwhile x\ne 0 \bdo (x:=x-1;y:=y-x)$\\
           $[x \ge 0 \w y=y_0 + \frac{(x_0-x)(x_0+x-1)}{2} \w x=0]$\hfill WHT,3,4
    \item $x\ge 0\w x=x_0 \w y=y_0 \Rightarrow x \ge 0 \w y=y_0 + \frac{(x_0-x)(x_0+x-1)}{2}$
    \item $[x\ge 0\w x=x_0 \w y=y_0]$\\
            $\bwhile x\ne 0 \bdo (x:=x-1;y:=y-x)$\\
            $[x \ge 0 \w y=y_0 + \frac{(x_0-x)(x_0+x-1)}{2} \w x=0]$\hfill SP,5,6
    \item $x \ge 0 \w y=y_0 + \frac{(x_0-x)(x_0+x-1)}{2} \w x=0 \Rightarrow y=y_0 + \frac{x_0(x_0-1)}{2}$
    \item $[x\ge 0\w x=x_0 \w y=y_0]$
            $\bwhile x\ne 0 \bdo (x:=x-1;y:=y-x)$
            $[y = y_0 + \frac{x_0(x_0-1)}{2} ]$       \hfill WC,7,8
\end{enumerate}


\end{document}